lib/core: Add lemmas on maps and words used in examples/loops

src/Rupicola/Lib/Core.v
@@ -11,11 +11,13 @@ Require Export bedrock2.Scalars.
 Require Export bedrock2.Syntax.
 Require Export bedrock2.WeakestPreconditionProperties.
 Require Export coqutil.dlet.
+Require Import coqutil.Decidable.
 Require Export coqutil.Map.Interface coqutil.Map.Properties coqutil.Map.SortedList.
 Require Export coqutil.Z.PushPullMod.
 Require Export coqutil.Tactics.Tactics.
 Require Export coqutil.Tactics.letexists.
 Require Export coqutil.Word.Interface coqutil.Word.Properties.
+Require coqutil.Map.SortedListString.
 Require bedrock2.ProgramLogic.
 
 Open Scope string_scope.
@@ -50,9 +52,8 @@ Module map.
             {map' : map.map key value'}
             {map_ok : map.ok map}
             {map'_ok : map.ok map'}
-            {key_eqb}
-            {key_eq_dec :
-               forall x y : key, BoolSpec (x = y) (x <> y) (key_eqb x y)}.
+            {key_eqb : key -> key -> bool}
+            {key_eq_dec : EqDecider key_eqb}.
 
     Lemma put_put_diff_comm k1 k2 v1 v2 m :
       k1 <> k2 ->
@@ -149,6 +150,176 @@ Module map.
       - intros; rewrite !map.get_put_dec; destruct key_eqb; eauto.
     Qed.
   End __.
+
+  Definition map_of_list' {K V} {map: map.map K V} (rev_bindings: list (K * V)) (acc: map) :=
+    List.fold_right (fun '(k, v) m => map.put m k v) acc rev_bindings.
+
+  Lemma of_list_is_fold_right' {K V} {map: map.map K V}:
+    forall bs acc,
+      (fix of_list (l : list (K * V)) : map :=
+         match l with
+         | [] => acc
+         | (k, v) :: l => map.put (of_list l) k v
+         end) bs =
+      map_of_list' bs acc.
+  Proof.
+    induction bs as [ | [k v] ]; cbn; intros.
+    - reflexivity.
+    - rewrite IHbs; reflexivity.
+  Qed.
+
+  Lemma of_list_is_fold_right {K V} {map: map.map K V}:
+    forall bs, map.of_list bs = map_of_list' bs map.empty.
+  Proof. intros; apply of_list_is_fold_right'. Qed.
+
+  Definition map_domains_diff {K V} {map: map.map K V} (m0 m1: map) :=
+    map.keys (map.fold (fun (m0: map) k _ => map.remove m0 k) m0 m1).
+
+  Definition map_eq {K V} {map0 map1: map.map K V}
+             {map_ok0: map.ok map0} {map_ok1: map.ok map1}
+             m0 m1 :=
+    (forall k, map.get (map := map0) m0 k = map.get (map := map1) m1 k).
+
+  Instance map_eq_refl {K V} {map: map.map K V} {map_ok: map.ok map} :
+    RelationClasses.Reflexive (@map_eq K V map map map_ok map_ok).
+  Proof. unfold map_eq; constructor; congruence. Qed.
+
+  Lemma eq_trans {K V}
+        {map0 map1 map2: map.map K V}
+        {map_ok0: map.ok map0} {map_ok1: map.ok map1} {map_ok2: map.ok map2} :
+    forall m0 m1 m2,
+      map_eq (map0 := map0) (map1 := map1) m0 m1 ->
+      map_eq (map0 := map1) (map1 := map2) m1 m2 ->
+      map_eq m0 m2.
+  Proof. unfold map_eq; congruence. Qed.
+
+  Lemma eq_sym {K V}
+        {map0 map1: map.map K V}
+        {map_ok0: map.ok map0} {map_ok1: map.ok map1} :
+    forall m0 m1,
+      map_eq (map0 := map0) (map1 := map1) m0 m1 ->
+      map_eq (map0 := map1) (map1 := map0) m1 m0.
+  Proof. unfold map_eq; congruence. Qed.
+
+  Lemma put_proper {K V}
+        {map0 map1: map.map K V}
+        {map_ok0: map.ok map0} {map_ok1: map.ok map1}
+        {key_eqb: K -> K -> bool}
+        {key_eq_dec : EqDecider key_eqb} :
+    forall k v (m0: map.rep (map := map0)) (m1: map.rep (map := map1)),
+      map_eq m0 m1 ->
+      map_eq (map.put m0 k v) (map.put m1 k v).
+  Proof.
+    intros * Heq k.
+    destruct (key_eqb k0 k) eqn:Hk;
+      [ eapply (Decidable.BoolSpec_true _ _ _ (key_eq_dec _ _)) in Hk |
+        eapply (Decidable.BoolSpec_false _ _ _ (key_eq_dec _ _)) in Hk ];
+      subst; rewrite ?map.get_put_same, ?map.get_put_diff; auto.
+  Qed.
+
+  Lemma remove_proper {K V}
+        {map0 map1: map.map K V}
+        {map_ok0: map.ok map0} {map_ok1: map.ok map1}
+        {key_eqb: K -> K -> bool}
+        {key_eq_dec : EqDecider key_eqb} :
+    forall k (m0: map.rep (map := map0)) (m1: map.rep (map := map1)),
+      map_eq m0 m1 ->
+      map_eq (map.remove m0 k) (map.remove m1 k).
+  Proof.
+    intros * Heq k.
+    destruct (key_eqb k0 k) eqn:Hk;
+      [ eapply (Decidable.BoolSpec_true _ _ _ (key_eq_dec _ _)) in Hk |
+        eapply (Decidable.BoolSpec_false _ _ _ (key_eq_dec _ _)) in Hk ];
+      subst; rewrite ?map.get_remove_same, ?map.get_remove_diff; auto.
+  Qed.
+
+  Definition remove_many {K V} {M: map.map K V} m (ks: list K) :=
+    List.fold_left map.remove ks m.
+
+  Lemma remove_many_proper {K V}
+        {map0 map1: map.map K V}
+        {map_ok0: map.ok map0} {map_ok1: map.ok map1}
+        {key_eqb: K -> K -> bool}
+        {key_eq_dec : EqDecider key_eqb} :
+    forall ks (m0: map.rep (map := map0)) (m1: map.rep (map := map1)),
+      map_eq m0 m1 ->
+      map_eq (remove_many m0 ks) (remove_many m1 ks).
+  Proof.
+    unfold remove_many; induction ks; simpl; intros.
+    - assumption.
+    - apply IHks, remove_proper; assumption.
+  Qed.
+
+  Lemma ext_rev  {K V} {map: map.map K V} {map_ok: map.ok map} :
+    forall m0 m1, m0 = m1 -> map_eq m0 m1.
+  Proof. intros; subst; reflexivity. Qed.
+
+  Lemma remove_many_concretize {K V}
+        {map0 map1: map.map K V}
+        {map_ok0: map.ok map0} {map_ok1: map.ok map1}
+        {key_eqb: K -> K -> bool}
+        {key_eq_dec : EqDecider key_eqb} :
+    forall (m0 m'0: map.rep (map := map0)) (m1 m'1: map.rep (map := map1)) ks,
+      map_eq m0 m1 ->
+      map_eq m'0 m'1 ->
+      remove_many m1 ks = m'1 ->
+      remove_many m0 ks = m'0.
+  Proof.
+    intros * Heq H'eq H1.
+    apply ext_rev in H1.
+    apply map.map_ext; change (map_eq (remove_many m0 ks) m'0).
+    eauto using @eq_trans, @remove_many_proper, @eq_sym.
+  Qed.
+
+  Lemma of_list_proper' {K V}
+        {map0 map1: map.map K V}
+        {map_ok0: map.ok map0} {map_ok1: map.ok map1}
+        {key_eqb: K -> K -> bool}
+        {key_eq_dec : EqDecider key_eqb} :
+    forall bs m0 m1,
+      map_eq (map0 := map0) (map1 := map1) m0 m1 ->
+      map_eq (map_of_list' bs m0)
+             (map_of_list' bs m1).
+  Proof.
+    induction bs as [ | (k & v) bs ]; simpl; intros.
+    - assumption.
+    - apply put_proper, IHbs; assumption.
+  Qed.
+
+  Lemma eq_empty {K V}:
+    forall {map0 map1: map.map K V}
+      {map_ok0: map.ok map0} {map_ok1: map.ok map1},
+      map_eq (map.empty (map := map0)) (map.empty (map := map1)).
+  Proof.
+    red; intros; rewrite !map.get_empty; reflexivity.
+  Qed.
+
+  Lemma of_list_proper {K V}
+        {map0 map1: map.map K V}
+        {map_ok0: map.ok map0} {map_ok1: map.ok map1}
+        {key_eqb: K -> K -> bool}
+        {key_eq_dec : EqDecider key_eqb} :
+    forall bs,
+      map_eq (map.of_list (map := map0) bs)
+             (map.of_list (map := map1) bs).
+  Proof.
+    intros; rewrite !of_list_is_fold_right;
+      apply of_list_proper', eq_empty.
+  Qed.
+
+  Lemma remove_many_diff {V} {map: map.map string V} {map_ok: map.ok map}:
+    let SM := SortedListString.map V in
+    let SM_ok := SortedListString.ok V in
+    forall (b0 b1: list (string * V)) ks,
+      let sb0 := map.of_list (map := SM) b0 in
+      let sb1 := map.of_list (map := SM) b1 in
+      ks = map_domains_diff sb0 sb1 -> (* Used for unification *)
+      remove_many sb0 ks = sb1 ->
+      remove_many (map.of_list (map := map) b0) ks = map.of_list b1.
+  Proof.
+    intros; eapply (remove_many_concretize (map0 := map) (map1 := SM)); eauto;
+      apply of_list_proper.
+  Qed.
 End map.
 
 Hint Rewrite @map.get_put_diff @map.get_put_same @map.put_put_same
@@ -205,8 +376,10 @@ Module word.
   Section __.
     Context {width} {word : Interface.word width} {ok : word.ok word}.
 
+    Open Scope Z_scope.
+
     Lemma wrap_small x :
-      (0 <= x < 2 ^ width)%Z ->
+      0 <= x < 2 ^ width ->
       word.wrap x = x.
     Proof. apply Z.mod_small. Qed.
 
@@ -215,6 +388,60 @@ Module word.
     Proof.
       destruct b; cbn [Z.b2z];
         auto using word.unsigned_of_Z_0, word.unsigned_of_Z_1.
+    Qed.
+
+    Lemma swrap_eq z :
+      word.swrap z = z ->
+      - 2 ^ (width - 1) <= z < 2 ^ (width - 1).
+    Proof.
+      unfold word.swrap; intros H.
+      pose proof word.half_modulus_pos.
+      apply (Z.add_cancel_r _ _ (2 ^ (width - 1))) in H.
+      ring_simplify in H.
+      apply Z.mod_small_iff in H.
+      + destruct H as [ H | H ]; rewrite (word.pow2_width_minus1 (word := word)) in H; lia.
+      + rewrite word.pow2_width_minus1; lia.
+    Qed.
+
+    Lemma signed_unsigned_dec w :
+      word.signed w =
+      if Z_lt_le_dec (word.unsigned w) (2 ^ (width - 1))
+      then word.unsigned w
+      else word.unsigned w - 2 ^ width.
+    Proof.
+      rewrite word.signed_eq_swrap_unsigned.
+      pose proof word.unsigned_range w.
+      destruct Z_lt_le_dec.
+      - apply word.swrap_inrange; lia.
+      - unfold word.swrap.
+        rewrite (word.pow2_width_minus1 (word := word)) in *.
+        pose proof word.half_modulus_pos.
+        rewrite <- Z_mod_plus_full with (b := -1).
+        rewrite Z.mod_small; [ | split ]; lia.
+    Qed.
+
+    Lemma signed_gz_unsigned_bounds w :
+      0 <= word.signed w <->
+      word.unsigned w < 2 ^ (width - 1).
+    Proof.
+      split; intro H; pose proof word.unsigned_range w.
+      - rewrite signed_unsigned_dec in H.
+        destruct Z_lt_le_dec in H.
+        + assumption.
+        + exfalso; lia.
+      - rewrite word.signed_eq_swrap_unsigned, word.swrap_inrange; lia.
+    Qed.
+
+    Lemma signed_gz_eq_unsigned w :
+      0 <= word.signed w ->
+      word.unsigned w = word.signed w.
+    Proof.
+      intros Hgz.
+      rewrite word.signed_eq_swrap_unsigned, word.swrap_inrange.
+      - reflexivity.
+      - pose proof word.unsigned_range w.
+        apply signed_gz_unsigned_bounds in Hgz.
+        lia.
     Qed.
   End __.
 End word.
